

Finding derivatives

1. Use limit definition

$$\lim_{h \rightarrow 0} \frac{f(x+h) - f(x)}{h} \quad \text{or} \quad \lim_{p \rightarrow x} \frac{f(p) - f(x)}{p - x}$$

2. Power rule

$$f(x) = x^n \quad f'(x) = nx^{n-1}$$

$$x^n \cdot x^m = x^{n+m}$$

$$(x^n)^m = x^{nm}$$

$$x^{-n} = \frac{1}{x^n}$$

$$\frac{x^n}{x^m} = x^{n-m}$$

$$\sqrt[n]{x^m} = x^{\frac{m}{n}}$$

$$\frac{1}{x^{-n}} = \frac{1}{\frac{1}{x^n}} = x^n$$

3. $f(x) = e^x \quad f'(x) = x^e e^x$

4. Product rule

$$\frac{d}{dx}(f(x) \cdot g(x)) = f(x)g'(x) + f'(x)g(x)$$

5. Quotient rule

$$\frac{d}{dx}\left(\frac{f(x)}{g(x)}\right) = \frac{g(x)f'(x) - g'(x)f(x)}{\underbrace{g(x)^2}_{\text{Denominator}}}$$

6. Derivative of trig functions

$$\frac{d}{dx} \sin(x) = \cos(x)$$

$$\frac{d}{dx} \csc(x) = -\csc(x) \cot(x)$$

$$\frac{d}{dx} \cos(x) = -\sin(x)$$

$$\frac{d}{dx} \sec(x) = \sec(x) \tan(x)$$

$$\frac{d}{dx} \tan(x) = \sec^2(x)$$

$$\frac{d}{dx} \cot(x) = -\csc^2(x)$$

7. Chain rule

$$\frac{d}{dx} f(g(x)) = f'(g(x)) g'(x)$$

Ex: $H(x) = \sqrt{x^2+1} = (x^2+1)^{\frac{1}{2}}$

$$\begin{aligned} H'(x) &= \frac{1}{2} (x^2+1)^{-\frac{1}{2}} \frac{d}{dx} (x^2+1) \\ &= \frac{1}{2} (x^2+1)^{-\frac{1}{2}} (2x) \end{aligned}$$

8. $f(x) = b^x$ where $b > 0$

$f'(x) = b^x \ln(b)$

9. Derivative of inverse trig functions

$$\frac{d}{dx}(\sin^{-1} x) = \frac{1}{\sqrt{1-x^2}}$$

$$\frac{d}{dx}(\csc^{-1} x) = -\frac{1}{x\sqrt{x^2-1}}$$

$$\frac{d}{dx}(\cos^{-1} x) = -\frac{1}{\sqrt{1-x^2}}$$

$$\frac{d}{dx}(\sec^{-1} x) = \frac{1}{x\sqrt{x^2-1}}$$

$$\frac{d}{dx}(\tan^{-1} x) = \frac{1}{1+x^2}$$

$$\frac{d}{dx}(\cot^{-1} x) = -\frac{1}{1+x^2}$$

10. Implicit differentiation

- Derive an equation without isolating y

Ex: $x^4 + y^4 = 16$ Find y'

Find y''

$$\frac{d}{dx}(x^4 + y^4) = \frac{d}{dx}(16)$$

$$\frac{d}{dx} y' = \frac{d}{dx} \left(-\frac{x^3}{y^3} \right)$$

$$4x^3 + 4y^3 y' = 0$$

$$4y^3 y' = -4x^3$$

$$y' = \frac{-4x^3}{4y^4} = -\frac{x^3}{y^4}$$

$$y'' = -\frac{y^3 \frac{d}{dx} x^3 - x^3 \frac{d}{dx} y^3}{(y^3)^2}$$

$$= -\frac{y^3 3x^2 - x^3 3y^2 y'}{y^6}$$

$$= -\frac{y^3 3x^2 - x^3 3y^2 \left(-\frac{x^3}{y^4} \right)}{y^6}$$

$$11. \frac{d}{dx}(\log_b x) = \frac{1}{x \ln b} \quad \frac{d}{dx} \ln x = \frac{1}{x}$$

12. Logarithmic differentiation

- Taking \ln of both sides to use its properties to simplify taking the derivative.

- Property of logs if $a \& b > 0$

$$\log(ab) = \log(a) + \log(b) \quad \log(a^n) = n \log(a)$$

$$\log\left(\frac{a}{b}\right) = \log(a) - \log(b) \quad \log_b(a) = \frac{\ln(a)}{\ln(b)}$$

- $\log_e = \ln$ is used instead of other bases because its derivative is simple.

- Ex:

$$\text{Differentiate } y = \frac{x^{\frac{3}{4}} \sqrt{x^2+1}}{(3x+2)^5}$$

$$\begin{aligned} \ln y &= \ln \left(\frac{x^{\frac{3}{4}} \sqrt{x^2+1}}{(3x+2)^5} \right) = \ln \left(x^{\frac{3}{4}} \sqrt{x^2+1} \right) - \ln (3x+2)^5 \\ &= \ln \left(x^{\frac{3}{4}} \right) + \ln \sqrt{x^2+1} - 5 \ln (3x+2) \\ &= \frac{3}{4} \ln x + \frac{1}{2} \ln (x^2+1) - 5 \ln (3x+2) \end{aligned}$$

$$\frac{d}{dx} \ln y = \frac{d}{dx} \left(\frac{3}{4} \ln x + \frac{1}{2} \ln (x^2+1) - 5 \ln (3x+2) \right)$$

$$\frac{1}{y} y' = \frac{3}{4x} + \frac{1}{2(x^2+1)} \frac{d}{dx} (x^2+1) - \frac{5}{3x+2} \frac{d}{dx} (3x+2)$$

$$y' = y \left(\frac{3}{4x} + \frac{x}{x^2+1} - \frac{15}{3x+2} \right)$$

↑ substitute for y if necessary